SP1Operations/AddOperation.lean
@@ -13,12 +13,12 @@ def spec
   (cols : AddOperation)
   (a : Word U16)
   (b : Word U16)
-  (is_real : U2) : Prop :=
-    is_real = U2.one →
+  (is_real : U1) : Prop :=
+    is_real = U1.one →
     a.toFin32_U16 + b.toFin32_U16 = cols.value.toFin32_U16
 
 def constraints (cols : AddOperation)
-    (a b : Word U16) (is_real : U2) : List SP1Constraint :=
+    (a b : Word U16) (is_real : U1) : List SP1Constraint :=
   [
     .assertZero (is_real * ((((a[0].val + b[0].val) - cols.value[0].val) + (0 : BabyBear)) * (2013235201 : BabyBear)) * (((((a[0].val + b[0].val) - cols.value[0].val) + 0) * 2013235201) - 1)),
     .assertZero (is_real * ((((a[1].val + b[1].val) - cols.value[1].val) + ((((a[0].val + b[0].val) - cols.value[0].val) + (0 : BabyBear)) * (2013235201 : BabyBear))) * (2013235201 : BabyBear)) * (((((a[1].val + b[1].val) - cols.value[1].val) + ((((a[0].val + b[0].val) - cols.value[0].val) + 0) * 2013235201)) * 2013235201) - 1))
@@ -28,7 +28,7 @@ def constraints'
     (cols : AddOperation)
     (a : Word U16)
     (b : Word U16)
-    (is_real : U2): Prop :=
+    (is_real : U1): Prop :=
   let carry0 : BabyBear := 0
   let carry1 : BabyBear := (a[0] + b[0] - cols.value[0] + carry0) * (baseInv : BabyBear)
   let carry2 : BabyBear := (a[1] + b[1] - cols.value[1] + carry1) * (baseInv : BabyBear)
@@ -39,7 +39,7 @@ def constraints_iff_constraints'
     (cols : AddOperation)
     (a : Word U16)
     (b : Word U16)
-    (is_real : U2) :
+    (is_real : U1) :
     constraintList_toProp (cols.constraints a b is_real) ↔ cols.constraints' a b is_real:= by
   simp [constraints, constraints']
 
@@ -47,7 +47,7 @@ theorem correct
   (cols : AddOperation)
   (a : Word U16)
   (b : Word U16)
-  (is_real : U2)
+  (is_real : U1)
   : cols.constraints' a b is_real → cols.spec a b is_real :=
     by
       intro ⟨q1, q2⟩
