SP1Operations/IsZeroOperation.lean
@@ -4,16 +4,16 @@ structure IsZeroOperation where
   /-- The inverse of the input. -/
   inverse : U16
   /-- Result indicating whether the input is 0. This equals `inverse * input == \ 0`. -/
-  result  : U2
+  result  : U1
 
 namespace IsZeroOperation
 
 def spec (cols : IsZeroOperation)
-    (a : U16) (is_real : U2) : Prop :=
+    (a : U16) (is_real : U1) : Prop :=
   is_real = 1 → (a = 0 ↔ cols.result = 1)
 
 def constraints (cols : IsZeroOperation)
-    (a : U16) (is_real : U2) : List (SP1Constraint) :=
+    (a : U16) (is_real : U1) : List (SP1Constraint) :=
   [
   .assertZero (is_real.val * ((1 - (cols.inverse.val * a.val)) - cols.result.val)),
   .assertZero (is_real.val * (cols.result.val * (cols.result.val - 1))),
@@ -22,7 +22,7 @@ def constraints (cols : IsZeroOperation)
   ]
 
 theorem correct (cols : IsZeroOperation)
-    (a : U16) (is_real : U2) :
+    (a : U16) (is_real : U1) :
     constraintList_toProp (cols.constraints a is_real) → cols.spec a is_real := by
   simp [constraints, spec, sub_eq_zero]
   aesop
